more

haskell/Polysemy/Free.hs
@@ -1,0 +1,29 @@
+module  Free
+    (   Free        (..) 
+    ,   Teletype    (..)    -- TODO: clean up
+    )   where
+
+import Control.Monad
+
+data Free f k
+    = Pure k
+    | Impure (f (Free f k)) 
+
+instance Functor f => Functor (Free f) where
+    fmap g (Pure a)    = Pure   $ g a
+    fmap g (Impure fa) = Impure $ fmap (fmap g) fa
+
+instance Functor f => Applicative (Free f) where
+    pure  = return 
+    (<*>) = ap
+
+instance Functor f => Monad (Free f) where
+    return = undefined
+    (>>=)  = undefined
+
+-- TODO: clean up
+data Teletype a
+    = WriteLine String a
+    | ReadLine (String -> a)
+
+
