haskell/Polysemy/Lab.hs
@@ -1,0 +1,18 @@
+module  Lab
+    (   main
+    )   where
+
+import Teletype
+
+main :: IO ()
+main = runTeletype prog
+--main = print . fst . runTeletypePurely ["john"] $ prog
+
+prog :: Teletype ()
+prog = do
+    writeLine "What is your name:"
+    s <- readLine 
+    writeLine $ "Hello " ++ s ++ " please to meet you."
+
+
+
