haskell/cfui/Components/Files.hs
@@ -1,0 +1,17 @@
+module  Components.Files
+    (
+    )   where
+
+import UI
+import Store
+import State
+import Console
+import Component
+
+_filesComponent :: Component IO (Store [String]) (State [String]) Console
+_filesComponent = Store render initStore where
+    initStore :: [String]
+    initStore = []
+
+    render :: [String] -> UI IO (State [String]) Console
+    render = undefined
