haskell/cfui/Pairing.hs
@@ -1,22 +1,25 @@
-{-# LANGUAGE RankNTypes             #-}
+{-# LANGUAGE InstanceSigs           #-}
 {-# LANGUAGE FunctionalDependencies #-}
-{-# LANGUAGE MultiParamTypeClasses  #-}
 
 module  Pairing
     (   Pairing     (..) 
-    ,   Sequence    (..)
     ,   move
     )   where
---type Pairing f g = forall a b. f (a -> b) -> g a -> b
 
 import Control.Comonad
 
 import Data.Functor.Identity
 
+import Store
+import State
 import Stream
+import Sequence
 
 class Pairing f g | f -> g, g -> f where
     pair :: (a -> b -> c) -> f a -> g b -> c
+
+move :: (Comonad w, Pairing m w) => w a -> m b -> w a
+move space movement = pair (const id) movement (duplicate space)
 
 instance Pairing Identity Identity where
     pair f (Identity a) (Identity b) = f a b
@@ -24,42 +27,23 @@ instance Pairing Identity Identity where
 instance Pairing ((->) a) ((,) a) where
     pair f g (a,b) = f (g a) b 
 
-_uncurry :: (a -> b -> c) -> (a, b) -> c
-_uncurry = pair ($)
-
-move :: (Comonad w, Pairing m w) => w a -> m b -> w a
-move space movement = pair (const id) movement (duplicate space)
-
-s0 :: Stream Integer
-s0 = naturals
-
-data Sequence a = End a | Next (Sequence a)
-
-instance Functor Sequence where
-    fmap f (End x)   = End (f x)
-    fmap f (Next xs) = Next (fmap f xs)  
-
--- This definition is consistent with 'ap', see coq file
-instance Applicative Sequence where
-    pure  = End
-    (<*>) (End f)   (End a)   = End (f a)
-    (<*>) (End f)   (Next as) = Next (fmap f as)
-    (<*>) (Next fs) x         = Next (fs <*> x)
-
-instance Monad Sequence where
-    return  = End
-    (>>=) (End a)   f   = f a
-    (>>=) (Next as) f   = Next (as >>= f)
-
-_ap :: (Monad m) => m (a -> b) -> m a -> m b
-_ap mf ma = mf >>= \f -> ma >>= \a -> return (f a)
-
 instance Pairing Sequence Stream where
     pair f (End a) (Cons b _) = f a b
     pair f (Next as) (Cons _ bs) = pair f as bs
+
+instance Pairing (State s) (Store s) where
+  pair :: (a -> b -> c) -> State s a -> Store s b -> c
+  pair op (State f) (Store g s) = let (a,s') = f s in op a (g s')
+
+_uncurry :: (a -> b -> c) -> (a, b) -> c
+_uncurry = pair ($)
+
+s0 :: Stream Integer
+s0 = naturals
 
 _s1 :: Stream Integer
 _s1 = move s0 (Next (End ()))
 
 _s2 :: Stream Integer
 _s2 = move s0 (Next (Next (End ())))
+
