haskell/cfui/Sequence.hs
@@ -1,0 +1,22 @@
+module  Sequence
+    (   Sequence    (..)
+    )   where
+
+import Control.Monad
+
+data Sequence a = End a | Next (Sequence a)
+
+instance Functor Sequence where
+    fmap f (End x)   = End (f x)
+    fmap f (Next xs) = Next (fmap f xs)  
+
+instance Applicative Sequence where
+    pure  = return
+    (<*>) = ap
+
+instance Monad Sequence where
+    return  = End
+    (>>=) (End a)   f   = f a
+    (>>=) (Next as) f   = Next (as >>= f)
+
+
