haskell/cfui/Store.hs
@@ -1,16 +1,10 @@
 {-# LANGUAGE InstanceSigs           #-}
-{-# LANGUAGE FlexibleInstances      #-}
-{-# LANGUAGE MultiParamTypeClasses  #-}
 
 module  Store
     (   Store (..)
-    ,   State (..)
     )   where
 
 import Control.Comonad
-
-import State
-import Pairing
 
 data Store s a = Store (s -> a) s
 
@@ -23,7 +17,4 @@ instance Comonad (Store s) where
   duplicate :: Store s a -> Store s (Store s a)   -- Just a reminder 
   duplicate (Store f s) = Store (Store f) s
 
-instance Pairing (State s) (Store s) where
-  pair :: (a -> b -> c) -> State s a -> Store s b -> c
-  pair op (State f) (Store g s) = let (a,s') = f s in op a (g s')
 
