lean/tutorials/tutorial6.lean
@@ -19,9 +19,40 @@ begin
     ... ≤ ϕ (max N N')  : by { apply id_le_extraction', assumption }
 end
 
+lemma extraction_tendsto_inf : extraction ϕ → ∀ N', ∃ N, ∀ n ≥ N, ϕ n ≥ N' :=
+begin
+  intros H₁ N', use N', intros n H₂, calc
+    ϕ n   ≥ n           : by { apply id_le_extraction', assumption }
+    ...   ≥ N'          : by assumption
+end
+
 variables {u : ℕ → ℝ} {a l : ℝ}
 
 lemma near_cluster : cluster_point u a → ∀ ε > 0, ∀ N, ∃ n ≥ N, |u n - a| ≤ ε :=
 begin
-  sorry
+  intros H₁ ε H₂ N, rcases H₁ with ⟨ϕ,H₁,H₃⟩,
+  specialize H₃ ε H₂, cases H₃ with N₁ H₃,
+  have H₄ : ∃ n ≥ N₁, ϕ n ≥ N, { apply extraction_ge, assumption },
+  rcases H₄ with ⟨n,H₄,H₅⟩,
+  use (ϕ n), split; try { assumption }, apply H₃, assumption
 end
+
+lemma subseq_tendsto_of_tendsto' :
+  seq_limit u l       →
+  extraction ϕ        →
+  seq_limit (u ∘ ϕ) l :=
+begin
+  intros H₁ H₂ ε H₃, specialize H₁ ε H₃, cases H₁ with N₁ H₁,
+  have H₄ : ∃ N, ∀ n, n ≥ N → ϕ n ≥ N₁,
+    { apply extraction_tendsto_inf, assumption },
+  cases H₄ with N H₄,
+  use N, intros n H₅, apply H₁, apply H₄, assumption
+end
+
+lemma cluster_limit : seq_limit u l → cluster_point u a → a = l :=
+begin
+  intros H₁ H₂, rcases H₂ with ⟨ϕ,H₂,H₃⟩,
+  have H₄: seq_limit (u ∘ ϕ) l, { apply subseq_tendsto_of_tendsto; assumption },
+  apply unique_limit; assumption
+end
+
